SearchAddends cleaner implementation

SearchAddends.dfy
@@ -46,69 +46,34 @@ predicate AreAddendsIndices(q: seq<int>, x: int, i: nat, j: nat)
 predicate HasAddendsInIndicesRange(q: seq<int>, x: int, i: nat, j: nat)
 	requires AreOreredIndices(q, i, j)
 {
-	exists i', j' :: i <= i' < j' <= j < |q| && AreAddendsIndices(q, x, i', j')
+	HasAddends(q[i..(j + 1)], x)
 }
 
 predicate LoopInv(q: seq<int>, x: int, i: nat, j: nat, sum: int)
 {
-	AreOreredIndices(q, i, j) && HasAddendsInIndicesRange(q, x, i, j) && AreAddendsIndices(q, sum, i, j)
+	AreOreredIndices(q, i, j) &&
+	HasAddendsInIndicesRange(q, x, i, j) &&
+	AreAddendsIndices(q, sum, i, j)
 }
 
-lemma {:verify true} HasAddendsOnEntry(q: seq<int>, x: int)
+lemma LoopInvWhenSumIsBigger(q: seq<int>, x: int, i: nat, j: nat, sum: int)
 	requires HasAddends(q, x)
-	ensures HasAddendsInIndicesRange(q, x, 0, |q| - 1)
+	requires Sorted(q)
+	requires sum > x;
+	requires LoopInv(q, x, i, j, sum)
+	ensures HasAddendsInIndicesRange(q, x, i, j - 1)
 {
-	calc {
-		HasAddends(q, x);
-		==
-		exists i, j :: 0 <= i < j < |q| && q[i] + q[j] == x;
-		== { assert forall i, j :: (0 <= i < j < |q|) ==> (0 <= i < j <= |q| - 1 < |q|); }
-		exists i, j :: 0 <= i < j <= |q| - 1 < |q| && q[i] + q[j] == x;
-		== {
-			// Extracting this to a lemma doesn't work for some reason
-			assert |q| > 1;
-			assert 0 <= 0 < |q|;
-			assert 0 <= |q| - 1 < |q|;
-			assert forall i, j :: 0 <= i < j <= |q| - 1 < |q| && q[i] + q[j] == x ==> AreAddendsIndices(q, x, i, j);
-		}
-		exists i, j :: 0 <= i < j <= |q| - 1 < |q| && AreAddendsIndices(q, x, i, j);
-		==
-		HasAddendsInIndicesRange(q, x, 0, |q| - 1);
-	}
-}
-
-lemma LoopInvOnEntry(q: seq<int>, x: int, i: nat, j: nat, sum: int)
-	requires sorted: Sorted(q)
-	requires hasAddends: HasAddends(q, x)
-	requires indices: i == 0 && j == |q| - 1
-	requires sum: sum == q[i] + q[j]
-	ensures LoopInv(q, x, i, j, sum)
-{
-	assert |q| > 1 by {
-		reveal hasAddends;
-	}
-	assert AreOreredIndices(q, i, j) by {
-		reveal indices;
-	}
-	assert HasAddendsInIndicesRange(q, x, i, j) by {
-		reveal hasAddends;
-		HasAddendsOnEntry(q, x);
-		reveal indices;
-	}
-	assert AreAddendsIndices(q, sum, i, j) by {
-		reveal sum;
-	}
+	assert q[i..j] < q[i..(j + 1)];
 }
 
 method FindAddends'(q: seq<int>, x: int) returns (i: nat, j: nat)
 	requires Sorted(q) && HasAddends(q, x)
-	ensures i < j < |q| && q[i] + q[j] == x
+	ensures i < j < |q| && q[i]+q[j] == x
 {
 	i := 0;
 	j := |q| - 1;
 	var sum := q[i] + q[j];
-	
-	LoopInvOnEntry(q, x, i, j, sum);
+
 	while sum != x
 		invariant LoopInv(q, x, i, j, sum)
 		decreases j - i
@@ -116,6 +81,7 @@ method FindAddends'(q: seq<int>, x: int) returns (i: nat, j: nat)
 		if (sum > x)
 		{
 			// Sum it too big, lower it by decreasing the high index
+			LoopInvWhenSumIsBigger(q, x, i, j, sum);
 			j := j - 1;
 		}
 		// 'sum == x' cannot occur because the loop's guard is 'sum !=x'.
@@ -136,8 +102,7 @@ method FindAddends(q: seq<int>, x: int) returns (i: nat, j: nat)
 	i := 0;
 	j := |q| - 1;
 	var sum := q[i] + q[j];
-	
-	LoopInvOnEntry(q, x, i, j, sum);
+
 	while sum != x
 		invariant LoopInv(q, x, i, j, sum)
 		decreases j - i
@@ -154,6 +119,7 @@ method FindAddends(q: seq<int>, x: int) returns (i: nat, j: nat)
 			assert LoopInv(q, x, i, j, sum); // from loop invariant
 			assert sum > x; // from the if guard
 			// ==>?
+			LoopInvWhenSumIsBigger(q, x, i, j, sum);
 			assert LoopInv(q, x, i, j - 1, q[i] + q[j - 1]);
 			j := j - 1;
 			assert LoopInv(q, x, i, j, q[i] + q[j]);
